lib_list/ArrayListGen.fsti
@@ -118,20 +118,22 @@ val intro_arraylist_nil (#a:Type) (#opened:inames)
     )
 
 /// If the head of one of the lists is not null, then it is in the list
-val lemma_head1_not_null_mem (#a:Type) (#opened:inames)
+val lemma_head_not_null_mem (#a:Type) (#opened:inames)
   (pred1 pred2 pred3: a -> prop)
   (r:A.array (cell a))
   (hd1 hd2 hd3:US.t) :
   SteelGhost unit opened
     (varraylist pred1 pred2 pred3 r (US.v hd1) (US.v hd2) (US.v hd3))
     (fun _ -> varraylist pred1 pred2 pred3 r (US.v hd1) (US.v hd2) (US.v hd3))
-    (requires fun _ -> hd1 <> null_ptr)
+    (requires fun _ -> True)
     (ensures fun h0 _ h1 ->
       // Framing
       h0 (varraylist pred1 pred2 pred3 r (US.v hd1) (US.v hd2) (US.v hd3)) ==
       h1 (varraylist pred1 pred2 pred3 r (US.v hd1) (US.v hd2) (US.v hd3)) /\
       // Functional property
-      mem (US.v hd1) (US.v hd1) (h1 (varraylist pred1 pred2 pred3 r (US.v hd1) (US.v hd2) (US.v hd3)))
+      (hd1 = null_ptr \/ mem (US.v hd1) (US.v hd1) (h1 (varraylist pred1 pred2 pred3 r (US.v hd1) (US.v hd2) (US.v hd3)))) /\
+      (hd2 = null_ptr \/ mem (US.v hd2) (US.v hd2) (h1 (varraylist pred1 pred2 pred3 r (US.v hd1) (US.v hd2) (US.v hd3)))) /\
+      (hd3 = null_ptr \/ mem (US.v hd3) (US.v hd3) (h1 (varraylist pred1 pred2 pred3 r (US.v hd1) (US.v hd2) (US.v hd3))))
     )
 
 /// If the head of one of the lists is not null, then it is smaller than the length
